Gset wip

Enable-wins_flag/App.fst
@@ -38,7 +38,7 @@ let do_s (s:concrete_st_s) (op:log_entry) : concrete_st_s =
   if snd op = Enable then true else false
 
 //equivalence relation between the concrete states of sequential type and MRDT
-let eq (st_s:concrete_st_s) (st:concrete_st) = st_s = snd st
+let eq (st_s:concrete_st_s) (st:concrete_st) = st_s == snd st
 
 //initial states are equivalent
 let initial_eq _
