Grow-only_set_wip/App.fst
@@ -2,38 +2,46 @@ module App
 
 open FStar.Seq
 open FStar.Ghost
+module L = FStar.List.Tot
 
+let rec unique_s (l:list nat) =
+  match l with
+  |[] -> true
+  |id::xs -> not (L.mem id xs) && unique_s xs
+  
 // the concrete state type
-// It is a pair of timestamp and value
-type concrete_st = nat & nat
+// It is a list of unique elements
+type concrete_st = l:list nat{unique_s l}
 
 //initial state
-let init_st = (0, 0)
+let init_st = []
 
 // operation type
-// (the only operation is Write value, so nat is fine)
+// (the only operation is Add, so nat is fine)
 type op_t = nat
 
 // concrete do pre-condition
 let concrete_do_pre _ _ = true
 
 // apply an operation to a state
-let do (s:concrete_st) (op:log_entry) : (r:concrete_st{r = op}) = op
+let do (s:concrete_st) (op:log_entry) : concrete_st = 
+  if (L.mem (snd op) s) then s else (snd op)::s
 
 ////////////////////////////////////////////////////////////////
 //// Sequential implementation //////
 
 // the concrete state 
-type concrete_st_s = nat
+type concrete_st_s = list nat
 
 // init state 
-let init_st_s = 0
+let init_st_s = []
 
 // apply an operation to a state 
-let do_s (s:concrete_st_s) (op:log_entry) : concrete_st_s = snd op
+let do_s (s:concrete_st_s) (op:log_entry) : concrete_st_s = snd op::s
 
 //equivalence relation between the concrete states of sequential type and MRDT
-let eq (st_s:concrete_st_s) (st:concrete_st) = st_s == snd st
+let eq (st_s:concrete_st_s) (st:concrete_st) = 
+  (forall e. L.mem e st_s <==> L.mem e st)
 
 //initial states are equivalent
 let initial_eq _
@@ -47,58 +55,81 @@ let do_eq (st_s:concrete_st_s) (st:concrete_st) (op:log_entry)
 
 ////////////////////////////////////////////////////////////////
 
+let rec mem_ele (e:nat) (l:log) : Tot bool (decreases length l) =
+  match length l with
+  |0 -> false
+  |_ -> snd (head l) = e || mem_ele e (tail l)
+  
 let rec lem_foldl (s:concrete_st) (l:log)
   : Lemma (requires foldl_prop s l)
-          (ensures (length l > 0 ==> (let _, last = un_snoc l in seq_foldl s l = last) /\
-                                     mem_id (fst (seq_foldl s l)) l) /\
-                   (length l = 0 ==> (seq_foldl s l = s)) /\
-                   (length l > 0 /\ (forall id. mem_id id l ==> lt (fst s) id) ==> (lt (fst s) (fst (seq_foldl s l)))))
+          (ensures (length l = 0 ==> s = seq_foldl s l) /\
+                   (forall e. L.mem e (seq_foldl s l) <==> L.mem e s \/ mem_ele e l))
           (decreases length l)
   = match length l with
     |0 -> ()
     |_ -> lem_foldl (do s (head l)) (tail l)
 
 //conflict resolution
-let resolve_conflict (x y:log_entry) : (l:log{forall e. mem e l <==> e = x \/ e = y}) =
-  if lt (fst y) (fst x)
-    then cons y (cons x empty)
-      else cons x (cons y empty)
-
-#push-options "--z3rlimit 50"
-let resolve_conflict_prop (x y:log_entry)
-  : Lemma (requires fst x <> fst y)
-          (ensures (lt (fst y) (fst x) <==> last (resolve_conflict x y) = x) /\
-                   (last (resolve_conflict x y) <> x <==> lt (fst x) (fst y)))
-  = ()
+let resolve_conflict (x y:log_entry) : log =
+  cons x (cons y empty)
 
 // concrete merge pre-condition
-let concrete_merge_pre lca a b : prop = true
+let concrete_merge_pre lca a b : prop = 
+  (forall e. L.mem e lca ==> L.mem e a /\ L.mem e b)
+
+let rec concrete_merge1 (lca:concrete_st) (s1:concrete_st) (s2:concrete_st) 
+  : Pure concrete_st (requires concrete_merge_pre lca s1 s2)
+                     (ensures (fun r -> (forall e. L.mem e r <==> L.mem e s1 \/ L.mem e s2)))
+                     (decreases %[lca; s1; s2]) = 
+  match lca, s1, s2 with
+    |[],[],[] -> []
+    |x::xs,_,_ -> concrete_merge1 xs s1 s2
+    |[],x::xs,_ -> if L.mem x s2 then (concrete_merge1 [] xs s2) 
+                    else x::(concrete_merge1 [] xs s2)
+    |[],[],_ -> s2
 
 // concrete merge operation
-let concrete_merge (lca:concrete_st) (s1:concrete_st) (s2:concrete_st{concrete_merge_pre lca s1 s2}) : concrete_st = 
-  if lt (fst s1) (fst s2) then s2 else s1
+let concrete_merge (lca:concrete_st) (s1:concrete_st) (s2:concrete_st{concrete_merge_pre lca s1 s2}) : concrete_st =
+  concrete_merge1 lca s1 s2
 
 let merge_prop (lca s1 s2:st)
   : Lemma (requires is_prefix (ops_of lca) (ops_of s1) /\ 
                     is_prefix (ops_of lca) (ops_of s2))
           (ensures concrete_merge_pre (v_of lca) (v_of s1) (v_of s2)) = 
-  ()
+  lem_foldl init_st (ops_of s1); 
+  lem_foldl init_st (ops_of s2);
+  split_prefix init_st (ops_of lca) (ops_of s1);
+  split_prefix init_st (ops_of lca) (ops_of s2);
+  lem_foldl (v_of lca) (diff (ops_of s1) (ops_of lca));
+  lem_foldl (v_of lca) (diff (ops_of s2) (ops_of lca))
 
 let merge_inv_s1_prop (lca s1 s2:st)
   : Lemma (requires is_prefix (ops_of lca) (ops_of s1) /\
                     is_prefix (ops_of lca) (ops_of s2) /\
                     length (ops_of s1) > length (ops_of lca))
           (ensures concrete_merge_pre (v_of lca) (v_of (inverse_st s1)) (v_of s2)) =
-  ()
+  lem_foldl init_st (ops_of s2); 
+  lem_foldl init_st (ops_of (inverse_st s1));
+  lem_inverse (ops_of lca) (ops_of s1);
+  split_prefix init_st (ops_of lca) (ops_of (inverse_st s1));
+  split_prefix init_st (ops_of lca) (ops_of s2);
+  lem_foldl (v_of lca) (diff (ops_of (inverse_st s1)) (ops_of lca));
+  lem_foldl (v_of lca) (diff (ops_of s2) (ops_of lca))
 
 let merge_inv_s2_prop (lca s1 s2:st)
   : Lemma (requires is_prefix (ops_of lca) (ops_of s1) /\
                     is_prefix (ops_of lca) (ops_of s2) /\
                     length (ops_of s2) > length (ops_of lca))
           (ensures concrete_merge_pre (v_of lca) (v_of s1) (v_of (inverse_st s2))) =
-  ()
+  lem_foldl init_st (ops_of s1);
+  lem_foldl init_st (ops_of (inverse_st s2));
+  lem_inverse (ops_of lca) (ops_of s2);
+  split_prefix init_st (ops_of lca) (ops_of (inverse_st s2));
+  split_prefix init_st (ops_of lca) (ops_of s1);
+  lem_foldl (v_of lca) (diff (ops_of (inverse_st s2)) (ops_of lca));
+  lem_foldl (v_of lca) (diff (ops_of s1) (ops_of lca))
 
-let linearizable_s1_0 (lca s1 s2:st)
+let linearizable_s1_01 (lca s1 s2:st)
   : Lemma 
       (requires concrete_merge_pre (v_of lca) (v_of s1) (v_of s2) /\
                 is_prefix (ops_of lca) (ops_of s1) /\
@@ -108,13 +139,15 @@ let linearizable_s1_0 (lca s1 s2:st)
                 (forall id id1. mem_id id (ops_of lca) /\ mem_id id1 (diff (ops_of s2) (ops_of lca)) ==> lt id id1) /\
                 (forall id. mem_id id (diff (ops_of s1) (ops_of lca)) ==> not (mem_id id (diff (ops_of s2) (ops_of lca)))) /\
                 foldl_prop (v_of lca) (diff (ops_of s2) (ops_of lca)))
-      (ensures concrete_merge (v_of lca) (v_of s1) (v_of s2) == 
-               seq_foldl (v_of lca) (diff (ops_of s2) (ops_of lca))) =
+      (ensures (forall e. L.mem e (concrete_merge (v_of lca) (v_of s1) (v_of s2)) <==>
+                     L.mem e (seq_foldl (v_of lca) (diff (ops_of s2) (ops_of lca))))) =
   lem_foldl init_st (ops_of lca);
+  lem_foldl init_st (ops_of s1);
   lem_foldl init_st (ops_of s2);
+  split_prefix init_st (ops_of lca) (ops_of s2);
   lem_foldl (v_of lca) (diff (ops_of s2) (ops_of lca))
   
-let linearizable_s2_0 (lca s1 s2:st)
+let linearizable_s2_01 (lca s1 s2:st)
   : Lemma 
       (requires concrete_merge_pre (v_of lca) (v_of s1) (v_of s2) /\
                 is_prefix (ops_of lca) (ops_of s1) /\
@@ -125,14 +158,33 @@ let linearizable_s2_0 (lca s1 s2:st)
                 (forall id id1. mem_id id (ops_of lca) /\ mem_id id1 (diff (ops_of s2) (ops_of lca)) ==> lt id id1) /\
                 (forall id. mem_id id (diff (ops_of s1) (ops_of lca)) ==> not (mem_id id (diff (ops_of s2) (ops_of lca)))) /\
                 foldl_prop (v_of lca) (diff (ops_of s1) (ops_of lca)))
-      (ensures concrete_merge (v_of lca) (v_of s1) (v_of s2) == 
-               seq_foldl (v_of lca) (diff (ops_of s1) (ops_of lca))) =
+      (ensures (forall e. L.mem e (concrete_merge (v_of lca) (v_of s1) (v_of s2)) <==>
+                     L.mem e (seq_foldl (v_of lca) (diff (ops_of s1) (ops_of lca))))) =
   lem_foldl init_st (ops_of lca);
   lem_foldl init_st (ops_of s1);
+  lem_foldl init_st (ops_of s2);
+  split_prefix init_st (ops_of lca) (ops_of s1);
   lem_foldl (v_of lca) (diff (ops_of s1) (ops_of lca))
 
-#push-options "--z3rlimit 100"
-let linearizable_s1_gt0 (lca s1 s2:st)
+let rec inverse_helper1 (s:concrete_st) (l':log) (op:log_entry)
+  : Lemma (requires foldl_prop s l' /\ concrete_do_pre (seq_foldl s l') op)
+          (ensures (let l = Seq.snoc l' op in
+                    foldl_prop s l /\
+                    seq_foldl s l == do (seq_foldl s l') op /\
+                    (forall e. L.mem e (seq_foldl s l) <==> L.mem e (seq_foldl s l') \/ e = snd op)))
+          (decreases length l')
+  = Seq.un_snoc_snoc l' op;
+    match length l' with
+    |0 -> ()
+    |1 -> ()
+    |_ -> inverse_helper1 (do s (head l')) (tail l') op
+
+let lem_do (s:concrete_st) (op:log_entry)
+  : Lemma (ensures (forall e. L.mem e (do s op) <==> L.mem e s \/ e = snd op))
+  = ()
+  
+#push-options "--z3rlimit 200"
+let linearizable_s1_gt01 (lca s1 s2:st)
   : Lemma (requires is_prefix (ops_of lca) (ops_of s1) /\
                     is_prefix (ops_of lca) (ops_of s2) /\
                     Seq.length (ops_of s1) > Seq.length (ops_of lca) /\ 
@@ -147,20 +199,25 @@ let linearizable_s1_gt0 (lca s1 s2:st)
                      let _, last2 = un_snoc (ops_of s2) in
                      last (resolve_conflict last1 last2) = last1))
           (ensures (let _, last1 = un_snoc (ops_of s1) in
-                   concrete_do_pre (concrete_merge (v_of lca) (v_of (inverse_st s1)) (v_of s2)) last1 /\
-                   concrete_merge (v_of lca) (v_of s1) (v_of s2) ==
-                   do (concrete_merge (v_of lca) (v_of (inverse_st s1)) (v_of s2)) last1)) =
-  let _, last1 = un_snoc (ops_of s1) in
+                  concrete_do_pre (concrete_merge (v_of lca) (v_of (inverse_st s1)) (v_of s2)) last1 /\
+                  (forall e. L.mem e (concrete_merge (v_of lca) (v_of s1) (v_of s2)) <==>
+                        L.mem e (do (concrete_merge (v_of lca) (v_of (inverse_st s1)) (v_of s2)) last1)))) =
+  let p1, last1 = un_snoc (ops_of s1) in
   let _, last2 = un_snoc (ops_of s2) in
+  inverse_helper1 init_st p1 last1;
+  split_prefix init_st (ops_of lca) (ops_of s1);
+  lem_foldl (v_of lca) (diff (ops_of s1) (ops_of lca));
+  lem_foldl init_st (ops_of s1);
+  lem_foldl init_st (ops_of s2);
   assert (concrete_do_pre (concrete_merge (v_of lca) (v_of (inverse_st s1)) (v_of s2)) last1);
-  lem_seq_foldl init_st (ops_of s1);
-  lem_seq_foldl init_st (ops_of s2);
-  lastop_neq (ops_of lca) (ops_of s1) (ops_of s2);
-  assert (fst last1 <> fst last2);
-  resolve_conflict_prop last1 last2;
-  lem_foldl init_st (ops_of s1)
+  assert (forall e. L.mem e (concrete_merge (v_of lca) (v_of s1) (v_of s2)) <==>
+               L.mem e (concrete_merge (v_of lca) (v_of (inverse_st s1)) (v_of s2)) \/ e = snd last1);
+  lem_do (concrete_merge (v_of lca) (v_of (inverse_st s1)) (v_of s2)) last1;
+  assert (forall e. L.mem e (concrete_merge (v_of lca) (v_of s1) (v_of s2)) <==>
+               L.mem e (do (concrete_merge (v_of lca) (v_of (inverse_st s1)) (v_of s2)) last1));
+  ()
 
-let linearizable_s2_gt0 (lca s1 s2:st)
+let linearizable_s2_gt01 (lca s1 s2:st)
   : Lemma (requires is_prefix (ops_of lca) (ops_of s1) /\
                     is_prefix (ops_of lca) (ops_of s2) /\
                     Seq.length (ops_of s1) > Seq.length (ops_of lca) /\ 
@@ -176,15 +233,20 @@ let linearizable_s2_gt0 (lca s1 s2:st)
                      last (resolve_conflict last1 last2) <> last1))
           (ensures (let _, last2 = un_snoc (ops_of s2) in
                    concrete_do_pre (concrete_merge (v_of lca) (v_of s1) (v_of (inverse_st s2))) last2 /\
-                   concrete_merge (v_of lca) (v_of s1) (v_of s2) ==
-                   do (concrete_merge (v_of lca) (v_of s1) (v_of (inverse_st s2))) last2)) =
+                   (forall e. L.mem e (concrete_merge (v_of lca) (v_of s1) (v_of s2)) <==>
+                         L.mem e (do (concrete_merge (v_of lca) (v_of s1) (v_of (inverse_st s2))) last2)))) =
   let _, last1 = un_snoc (ops_of s1) in
-  let _, last2 = un_snoc (ops_of s2) in
-  assert (concrete_do_pre (concrete_merge (v_of lca) (v_of s1) (v_of (inverse_st s2))) last2);
-  lem_seq_foldl init_st (ops_of s1);
-  lem_seq_foldl init_st (ops_of s2);
-  lastop_neq (ops_of lca) (ops_of s1) (ops_of s2);
-  assert (fst last1 <> fst last2); 
-  resolve_conflict_prop last1 last2;
-  lem_foldl init_st (ops_of s2)
+  let p2, last2 = un_snoc (ops_of s2) in
+  inverse_helper1 init_st p2 last2;
+  split_prefix init_st (ops_of lca) (ops_of s2);
+  lem_foldl (v_of lca) (diff (ops_of s2) (ops_of lca));
+  lem_foldl init_st (ops_of s1);
+  lem_foldl init_st (ops_of s2);
+  assert (concrete_do_pre (concrete_merge (v_of lca) (v_of s1) (v_of (inverse_st s2))) last2); 
+  assert (forall e. L.mem e (concrete_merge (v_of lca) (v_of s1) (v_of s2)) <==>
+               L.mem e (concrete_merge (v_of lca) (v_of s1) (v_of (inverse_st s2))) \/ e = snd last2);
+  lem_do (concrete_merge (v_of lca) (v_of s1) (v_of (inverse_st s2))) last2;
+  assert (forall e. L.mem e (concrete_merge (v_of lca) (v_of s1) (v_of s2)) <==>
+               L.mem e (do (concrete_merge (v_of lca) (v_of s1) (v_of (inverse_st s2))) last2));
+  ()
 #pop-options
