Append-only_log_wip/App.fst
@@ -1,0 +1,164 @@
+module App
+
+open FStar.Seq
+open FStar.Ghost
+module L = FStar.List.Tot
+
+let rec mem_id_s (id:nat) (l:list (nat * string)) =
+  match l with
+  |[] -> false
+  |(id1,_)::xs -> id = id1 || mem_id_s id xs
+
+let rec pos (ele:(nat * string)) (l:list(nat * string){L.mem ele l}) =
+  match l with
+  |ele1::xs -> if ele1 = ele then 0 else 1 + pos ele xs
+  
+let rec total_order (l:list (nat * string)) =
+  match l with
+  |[] | [_] -> True
+  |x::y::xs -> lt (fst y) (fst x) /\ total_order (y::xs)
+
+let ord (id:(nat * string)) (id1:(nat * string)) 
+        (l:list (nat * string) {L.mem id l /\ L.mem id1 l /\ total_order l}) = 
+  pos id l < pos id1 l 
+
+// the concrete state type
+// It is a list of pairs of timestamp and message ordered in descending order of timestamps
+type concrete_st = l:list (nat (*timestamp*) * string (*message*)) {total_order l}
+
+//initial state
+let init_st = []
+
+// operation type
+// (the only operation is append value, so string is fine)
+type op_t = string
+
+// concrete do pre-condition
+let concrete_do_pre (s:concrete_st) (op:log_entry) = 
+  L.length s > 0 ==> lt (fst (L.hd s)) (fst op)
+ // (forall e. L.mem e s ==> lt (fst e) (fst op))
+
+// apply an operation to a state
+let do (s:concrete_st) (op:log_entry{concrete_do_pre s op}) = op::s
+
+let rec mem_str_s (str:string) (l:list (nat * string)) =
+  match l with
+  |[] -> false
+  |(_,m)::xs -> str = m || mem_str_s str xs
+  
+////////////////////////////////////////////////////////////////
+//// Sequential implementation //////
+
+// the concrete state 
+type concrete_st_s = list string
+
+// init state 
+let init_st_s = []
+
+// apply an operation to a state 
+let do_s (s:concrete_st_s) (op:log_entry) : concrete_st_s = snd op::s
+
+//equivalence relation between the concrete states of sequential type and MRDT
+let eq (st_s:concrete_st_s) (st:concrete_st) =
+  (forall e. L.mem e st_s <==> mem_str_s e st)
+
+//initial states are equivalent
+let initial_eq _
+  : Lemma (ensures eq init_st_s init_st) = ()
+
+//equivalence between states of sequential type and MRDT at every operation
+let do_eq (st_s:concrete_st_s) (st:concrete_st) (op:log_entry)
+  : Lemma (requires eq st_s st /\ concrete_do_pre st op)
+          (ensures eq (do_s st_s op) (do st op)) 
+  = ()
+
+////////////////////////////////////////////////////////////////
+
+let rec lem_foldl (s:concrete_st) (l:log)
+  : Lemma (requires foldl_prop s l)
+          (ensures (length l = 0 ==> (seq_foldl s l = s)) /\
+                   (*length l > 0 ==> (forall id id1. mem_id id l /\ mem_id_s id1 s ==> lt id1 id)) /\*)
+                    total_order (seq_foldl s l))
+          (decreases length l)
+  = match length l with
+    |0 -> ()
+    |_ -> lem_foldl (do s (head l)) (tail l)
+
+//conflict resolution
+let resolve_conflict (x y:log_entry) : (l:log{forall e. mem e l <==> e = x \/ e = y}) =
+  if lt (fst y) (fst x)
+    then cons y (cons x empty)
+      else cons x (cons y empty)
+
+#push-options "--z3rlimit 50"
+let resolve_conflict_prop (x y:log_entry)
+  : Lemma (requires fst x <> fst y)
+          (ensures (lt (fst y) (fst x) <==> last (resolve_conflict x y) = x) /\
+                   (last (resolve_conflict x y) <> x <==> lt (fst x) (fst y)))
+  = ()
+
+let rec remove (x:(nat * string)) (s:concrete_st)
+  : Pure concrete_st
+    (requires L.mem x s)
+    (ensures (fun r -> (forall e. L.mem e r <==> L.mem e s /\ e <> x) /\ not (mem_id_s (fst x) r) /\
+                    (forall id. mem_id_s id r <==> mem_id_s id s /\ id <> fst x) /\
+                    (forall e e1. L.mem e r /\ L.mem e1 r /\ lt (fst e1) (fst e) /\ ord e e1 r <==>
+                             L.mem e s /\ L.mem e1 s /\ lt (fst e1) (fst e) /\ ord e e1 s /\ e <> x /\ e1 <> x))) =
+  match s with
+  |x1::xs -> if x = x1 then xs else x1::(remove x xs)
+
+let rec diff_s (a:concrete_st) (l:concrete_st)
+  : Pure concrete_st
+    (requires (forall e. L.mem e l ==> L.mem e a))
+    (ensures (fun r -> (forall e. L.mem e r <==> L.mem e a /\ not (L.mem e l)) /\
+                    (forall id. mem_id_s id r <==> mem_id_s id a /\ not (mem_id_s id l)) /\
+                    (forall e e1. L.mem e r /\ L.mem e1 r /\ lt (fst e1) (fst e) /\ ord e e1 r <==>
+             L.mem e a /\ L.mem e1 a /\ not (L.mem e l) /\ not (L.mem e1 l) /\ lt (fst e1) (fst e) /\ ord e e1 a)))
+    (decreases l) = 
+  match l with
+  |[] -> a
+  |x::xs -> diff_s (remove x a) xs
+
+#push-options "--z3rlimit 100"
+let rec union_s (a:concrete_st) (b:concrete_st)
+  : Pure concrete_st
+    (requires (forall e. L.mem e a ==> not (mem_id_s (fst e) b)) /\ 
+              (forall e. L.mem e b ==> not (mem_id_s (fst e) a)))
+    (ensures (fun u -> (forall e. L.mem e u <==> L.mem e a \/ L.mem e b)/\
+                    (forall e e1. ((L.mem e a /\ L.mem e1 a /\ lt (fst e1) (fst e) /\ ord e e1 a) \/
+                              (L.mem e b /\ L.mem e1 b /\ lt (fst e1) (fst e) /\ ord e e1 b) \/
+                              (L.mem e a /\ L.mem e1 b /\ lt (fst e1) (fst e)) \/
+                              (L.mem e b /\ L.mem e1 a /\ lt (fst e1) (fst e))) <==>
+                              (L.mem e u /\ L.mem e1 u /\ lt (fst e1) (fst e) /\ ord e e1 u)) /\
+                              (forall id. mem_id_s id u <==> mem_id_s id a \/ mem_id_s id b))) =
+  match a, b with
+  |[], [] -> []
+  |[], _ -> b
+  |_, [] -> a
+  |h1::t1, h2::t2 -> if lt (fst h2) (fst h1) then h1::(union_s t1 b) else h2::(union_s a t2)
+#pop-options
+
+// concrete merge pre-condition
+let concrete_merge_pre lca a b = 
+  forallb (fun e -> L.mem e a && L.mem e b) lca /\
+  forallb (fun e -> not (mem_id_s (fst e) (diff_s b lca))) (diff_s a lca) /\
+  forallb (fun e -> not (mem_id_s (fst e) (diff_s a lca))) (diff_s b lca)
+
+// concrete merge operation
+let concrete_merge (lca:concrete_st) (s1:concrete_st) (s2:concrete_st{concrete_merge_pre lca s1 s2}) 
+  : (r:concrete_st{(forall e. L.mem e r <==> L.mem e s1 \/ L.mem e s2) /\
+                   (forall e e1. (L.mem e r /\ L.mem e1 r /\ fst e > fst e1 /\ ord e e1 r) <==>
+                            (L.mem e lca /\ L.mem e1 lca /\ fst e > fst e1 /\ ord e e1 lca) \/
+                       (L.mem e (diff_s s1 lca) /\ L.mem e1 (diff_s s1 lca) /\ lt (fst e1) (fst e) /\ ord e e1 (diff_s s1 lca)) \/
+                       (L.mem e (diff_s s2 lca) /\ L.mem e1 (diff_s s2 lca) /\ lt (fst e1) (fst e) /\ ord e e1 (diff_s s2 lca)) \/
+                       (L.mem e (diff_s s1 lca) /\ L.mem e1 (diff_s s2 lca) /\ lt (fst e1) (fst e)) \/
+                       (L.mem e (diff_s s2 lca) /\ L.mem e1 (diff_s s1 lca) /\ lt (fst e1) (fst e)) \/
+                       (L.mem e (diff_s s1 lca) /\ L.mem e1 lca /\ lt (fst e1) (fst e)) \/
+                       (L.mem e (diff_s s2 lca) /\ L.mem e1 lca /\ lt (fst e1) (fst e)) \/
+                       (L.mem e lca /\ L.mem e1 (diff_s s1 lca) /\ lt (fst e1) (fst e)) \/
+                       (L.mem e lca /\ L.mem e1 (diff_s s2 lca) /\ lt (fst e1) (fst e)))}) = 
+  let la = diff_s s1 lca in
+  let lb = diff_s s2 lca in
+  let u = union_s la lb in 
+  let r = union_s u lca in 
+  r
